���D�G�ξ��v���z 

���z 1.3: $P(A1 \cup A2) = P(A1) + P(A2) \; ; \; if \; A1 \cap A2 = \emptyset$ 
���z 2.3: $P(E_1 \cup E_2 \cup \cdots) = \sum P(E_i)$

�ХΤ��z�t�� 1 �P���X�שw�z�ҩ����z 2.3�C

�ҩ��G

�� $A_i \cap A_j=\emptyset ; i \neq j$ �ɡA�ھڤ��z 1.3  $P(A_i \cup A_j) = P(A_i) + P(A_j)$�A

���O�i���צp�U�G

$P(E_1 \cup E_2 \cup E_3 \cdots) = P(E_1 \cup (E_2 \cup E_3 \cdots))=P(E_1)+P(E_2 \cup E_3 \cdots)$ ; �M�Τ��z 1.3, $A1=E_1, A2=(E_2 \cup E_3 \cdots)

$=P(E_1)+P(E_2)+P(E_3 \cdots) = ... = \sum P(E_i)$

�ҩ�����!


